theories/case_studies/ghost.v
@@ -1,0 +1,52 @@
+From stdpp Require Import list.
+
+(* Hazel Reasoning *)
+From program_logic Require Import state_reasoning.
+
+From iris.proofmode Require Import base tactics.
+From iris.algebra Require Import excl_auth.
+
+Section ghost_theory.
+  Context {A : Type}.
+
+  (* We use ghost variables with contents in the CMRA [Auth(Ex(List A))]. *)
+  Context `{!inG Σ (excl_authR (leibnizO (list A)))}.
+
+  (* The assertion [own γ (●E Ys)] states that the handler
+     has seen the elements [Ys]. *)
+  Definition handlerView γ Ys : iProp Σ :=
+    own γ (●E (Ys : ofe_car (leibnizO (list A)))).
+  (* The assertion [own γ (◯E Xs)] states that [iter]
+     has seen the elements [Xs]. *)
+  Definition iterView γ Xs : iProp Σ :=
+    own γ (◯E (Xs : ofe_car (leibnizO (list A)))).
+
+  (* Create a new ghost cell from this CMRA. *)
+  (* In the verification of [invert], the ghost variable [γ]
+     initially holds the empty list. *)
+  Lemma new_cell Zs : ⊢ (|==> ∃ γ, handlerView γ Zs ∗ iterView γ Zs)%I.
+  Proof.
+    iMod (own_alloc ((●E (Zs : ofe_car (leibnizO (list A)))) ⋅
+                     (◯E (Zs : ofe_car (leibnizO (list A)))))) as (γ) "[??]";
+    [ apply excl_auth_valid | eauto with iFrame ]; done.
+  Qed.
+
+  (* Handler and [iter]'s views are in agreement. *)
+  Lemma confront_views γ Ys Xs :
+    handlerView γ Ys -∗ iterView γ Xs -∗ ⌜ Xs = Ys ⌝.
+  Proof.
+    iIntros "Hγ● Hγ◯".
+    by iDestruct (own_valid_2 with "Hγ● Hγ◯") as %?%excl_auth_agree_L.
+  Qed.
+
+  (* With the ownership of both views, one can update the contents of [γ]. *)
+  Lemma update_cell γ Zs Ys Xs :
+    handlerView γ Ys -∗ iterView γ Xs ==∗ handlerView γ Zs  ∗ iterView γ Zs.
+  Proof.
+    iIntros "Hγ● Hγ◯".
+    iMod (own_update_2 _ _ _ (●E (Zs : ofe_car (leibnizO (list A))) ⋅
+                              ◯E (Zs : ofe_car (leibnizO (list A))))
+      with "Hγ● Hγ◯") as "[$$]";
+    [ apply excl_auth_update |]; done.
+  Qed.
+End ghost_theory.
