theories/case_studies/iterator.v
@@ -1,0 +1,91 @@
+
+From iris.proofmode Require Import base tactics.
+
+(* Hazel Reasoning *)
+From program_logic Require Import weakest_precondition 
+                                  tactics 
+                                  shallow_handler_reasoning 
+                                  deep_handler_reasoning 
+                                  state_reasoning.
+
+(* Local imports *)
+From affine_tes.lang Require Import hazel.
+From affine_tes.case_studies Require Import representable.
+
+
+Section iterator.
+  Context `{!heapGS Σ}.
+
+  Context {G : Type → Type} `{DataStructure Σ G, Iterable G}.
+  Context {A : Type} `{Representable Σ A}.
+  
+  Definition isIter (iter : val) (T : G A) : iProp Σ :=
+    ∀ Ψ (f : val) I,
+      □ (∀ us u v, ⌜permitted T (us ++ [u])⌝ -∗ 
+                   represents v u -∗
+                   I us -∗ 
+               EWP (f v) <| Ψ |> {{ _, I (us ++ [u]) }}) -∗
+      I [] -∗
+      EWP (iter <_> f) <| Ψ |> {{ _, ∃ us, ⌜complete T us⌝ ∗ I us }}.
+
+End iterator.
+
+Section list_iterator.
+
+  Context `{!heapGS Σ}.
+
+  Definition list_iter :=
+      (λ: "xs",
+        (Λ: (λ: "f", 
+              (rec: "go" "xs" := 
+                list-match: "xs" with
+                  CONS "x" => "xxs" => ("f" "x" ;; "go" (Load "xxs"))
+                | NIL => #()
+                end) "xs"
+           ))
+      )%V.
+
+  Lemma list_iter_go_helper A `{Representable Σ A} Ψ l I T (f : val) xs :
+    □ (∀ us u v,
+        ⌜permitted (l ++ T) (us ++ [u])⌝ -∗
+        represents v u -∗ I us -∗ EWP f v <| Ψ |> {{ _, I (us ++ [u]) }})%I -∗
+     I l -∗ represents xs T -∗
+    (EWP (rec: "go" "xs" :=
+              list-match: "xs" with
+                CONS "x" => "xxs" => (f "x" ;; "go" (Load "xxs"))
+              | NIL => #()
+           end)%V xs <| Ψ |> {{ _, ∃ us : list A, ⌜complete (l ++ T) us⌝ ∗ I us }})%I.
+  Proof.
+    iLöb as "IH" forall (l T xs); simpl.
+    iIntros "#Hf HIl Hrepr"; destruct T; simpl.
+    - iDestruct "Hrepr" as "->". rewrite /rec_unfold. ewp_pure_steps.
+      iExists l. iIntros "{$HIl} !%". by rewrite app_nil_r.
+    - iDestruct "Hrepr" as "(%x & %tl & %tlv & Hrepr & -> & Htl & Hrepr')".
+      rewrite -{1}/(represents tlv T). 
+      ewp_pure_steps. rewrite /rec_unfold. ewp_pure_steps. ewp_bind_rule. 
+      iApply (ewp_mono with "[Hf Hrepr HIl]").   
+      { iApply ("Hf" with "[] Hrepr HIl").
+        iPureIntro. exists T.  rewrite -app_assoc. done. }
+      iIntros (v) "HI !> /=". ewp_pure_steps.
+      ewp_bind_rule. iApply (ewp_load with "Htl").
+      iIntros "!> Htl !> /=".
+      iSpecialize ("IH" $! (l ++ [a]) T tlv).
+      rewrite -{2}app_assoc. simpl.
+      iApply ("IH" with "[] HI Hrepr'").
+      rewrite -{2}app_assoc. simpl. iApply "Hf".
+  Qed.
+
+  Lemma list_iter_isIter {A} `{Representable Σ A} (xs : val)  (T : list A) :
+    represents xs T -∗ EWP list_iter xs {{ i, isIter i T }}.
+  Proof.
+    iIntros "Hrepr". rewrite /list_iter. ewp_pure_steps. 
+    rewrite /isIter. 
+    iIntros (Ψ f I) "#Hf HI". 
+    do 4 ewp_value_or_step. iApply (ewp_bind [AppLCtx _]); first done.
+    do 2 ewp_value_or_step.
+    assert (HTeq : T = [] ++ T) by done.
+    rewrite {1 3}HTeq.
+    iApply (list_iter_go_helper _ Ψ [] I T f xs with "Hf HI Hrepr").
+  Qed. 
+
+End list_iterator.
